## 4.1 Subgroups

> [!definition] Definition 4.1.1: A subgroup $H$ (p91)
> Let $H \subseteq G$ be a subset of $G$. Then $H$ is called a _subgroup_ of $(G, \cdot)$ if the following properties are satisfied:
>
> 1. $e \in H$ (where $e$ is the identity element of $G$).
> 2. For any $f \in H$, also $f^{-1} \in H$.
> 3. For any $f, g \in H$, also $f \cdot g \in H$.

A subgroup $H \subseteq G$ inherits the group operation $\cdot$ from the larger group $(G, \cdot)$

-   So the group operation in $H$ is the **restriction** of the group operation of $G$
-   The third property in the definition makes sure that this operation sends two elements of $H$ to another element of $H$

> [!lemma] Lemma 4.1.2: When is a subset a subgroup? (p91)
> Let $(G, \cdot)$ be a group and let $H \subseteq G$ be a **non-empty** subset. Then $$H \text{ is a subgroup of } (G, \cdot) \iff \forall f, g \in H : \boxed{f \cdot g^{-1} \in H}$$

_Example 1_

The set of **even integers**,
$$ \boxed{2\mathbb{Z}} = \{\ldots, -4, -2, 0 = e, 2, 4, \ldots\},$$
is a subgroup of the group of integers $(\mathbb{Z}, +)$ according to the above Lemma 4.1.2:

-   Choose $k,\ell \in 2\mathbb{Z}$.
-   Since $k$ and $\ell$ are even numbers, $k - \ell$ is an even number as well.
-   This implies $$k-\ell \in 2\mathbb{Z} \quad \overset{\Delta}{\Leftrightarrow} \quad k \cdot \ell^{-1} \in 2\mathbb{Z} \quad \overset{\text{Lemma 4.1.2}}{\iff} \quad 2\mathbb{Z} \text{ is a subgroup of } (\mathbb{Z}, +)$$

_Example 2_

The cycling group $C_n = \{e, g, g^2, \ldots, g^{n-1}\}$ is a subgroup of the dihedral group $(D_n, \circ)$.\
We can show this by using Definition 4.1.1:

1. The identity element $e$ of $D_n$ is also in $C_n$.
2. If $r^i \in C_n$, then $(r^i)^{-1} = r^{(-i) \bmod n} \in C_n$. (Lemma 3.2.1)
3. If $r^i, r^j \in C_n$, then $r^i \circ r^j = r^{(i+j) \bmod n} \in C_n$. (Lemma 3.2.1)

> [!definition] Definition 4.1.7: The subgroup generated by an element (p92)
> Let $(G, \cdot)$ be a group and let $g \in G$ be a group element. The set
> $$\gen{g} = \{g^i \mid i \in \mathbb{Z}\}$$
> is a subgroup of $G$, and is said to be the **subgroup generated by $g$**.

Note that $\gen{g}$ is indeed a subgroup, by Definition 4.1.1:

1. $e = g^0 \in \gen{g}$
2. If $f = g^i \in \gen{g}$, then $f^{-1} = (g^i)^{-1} = g^{-i} \in \gen{g}$
3. If $g^i,g^j \in \gen{g}$, then $g^i \cdot g^j = g^{i+j} \in \gen{g}$

> [!lemma] Lemma 4.1.8: Order of the subgroup $\gen{g}$ (p92)
> Let $(G, \cdot)$ be a group and let $g \in G$ be a group element. Then
> $$\boxed{|\gen{g}| = \operatorname{ord}(g)}$$
> So the order of the subgroup $\gen{g}$ is the same as the order of the element $g$.

> [!theorem]
> Let $\gen{g}$ be the subgroup generated by an element $g$ of a group $(G, \cdot)$ and let $\operatorname{ord}(g) = n < \infty$. Then:
> $$\forall i\in \Z : \boxed{g^i = g^{i \bmod n}} \quad \Rightarrow g^n = e$$

Using division with remainder, we can write any integer $i$:
$$i \quad = \quad n \cdot (i \operatorname{quot} n) + (i \bmod n) \quad = \quad n \cdot q + (i \bmod n)$$
Then it holds that

$$
\begin{align}
g^i &= g^{q \cdot n + (i \bmod n)} \\
&= g^{q \cdot n} \cdot g^{(i \bmod n)} \\
&= (g^n)^q \cdot g^{(i \bmod n)} \\
&= e^q \cdot g^{(i \bmod n)} \\
&= g^{(i \bmod n)}
\end{align}
$$

---

Note that for the group $(\Z, +)$, we have $$\boxed{n \Z = \gen{n}} = \{ \ldots, -2n, -n, 0, n, 2n, \ldots \}$$and that this is a **subgroup** of $(\Z, +)$.

In week 1, we saw that the congruence class of $a \in \Z$ modulo $n$ is defined as
$$a + n\Z = \{ a + k \cdot n \mid k \in \Z \}$$
This is exactly the same as the **coset** $a + \gen{n}$ of the subgroup $\gen{n} = n\Z$ of the group $(\Z, +)$.

## 4.2 Cosets of a group

> [!definition] Definition 4.2.1: Multiplication of subsets (p93)
> Let $(G, \cdot)$ be a group and let $M \subseteq G$ and $N \subseteq G$ be two subsets of $G$. Then we define
> $$M \cdot N = \{ f \cdot g \mid f \in M, g \in N \}$$

Note that for $(\Z, +)$, this definition corresponds to the usual addition of sets:
$$M + N = \{ m + n \mid m \in M, n \in N \}$$

> [!definition] Definition 4.2.3: Left and right cosets (p93)
> Let $H$ be a subgroup of a group $(G, \cdot)$ and let $f \in G$ be a group element. Then we define the **left coset of $H$ in $G$ by $f$** as
> $$f \cdot H := \{f\} \cdot H = \{ f \cdot h \mid h \in H \}$$
> Similarly, we define the **right coset of $H$ in $G$ by $f$** as
> $$H \cdot f := H \cdot \{f\} = \{ h \cdot f \mid h \in H \}$$

> [!definition] Normal subgroup (HW2)
> A subgroup $H$ of a group $G$ is called a **normal subgroup** if
> $$\forall g \in G : gH = Hg$$
> Or in other words, if all left cosets of $H$ in $G$ are equal to the corresponding right cosets.

In an Abelian group, there is **no difference between left and right cosets** since $f \cdot h = h \cdot f$ for any $f,h \in G$.

> [!deduction]
> In an **Abelian** group, we can simply talk about cosets of $H$ in $G$ by $f$, without specifying left or right.
> Furthermore, in an Abelian group, **every subgroup is a normal subgroup**.

> [!notation] Notation: The set of all cosets of a subgroup in a group (p94)
> The set of **all _left_ cosets of $H$ in $G$** is denoted by
> $$G / H = \{ f \cdot H \mid f \in G \}$$
> Similarly, the set of **all _right_ cosets of $H$ in $G$** is denoted by
> $$H \backslash G = \{ H \cdot f \mid f \in G \}$$

> [!exercise] Exercise 4.19: Intersection is a subgroup
> The **intersection** of two subgroups is also **a subgroup**.

## 4.3 Cosets as equivalence classes

> [!definition] Definition 4.3.1: The relation $\sim_H$ (p95)
> Let $(G, \cdot)$ be a group and $H \subseteq G$ a subgroup. For $f, g \in G$, we write
>
> -   $\boxed{f \sim_H g  \quad \iff \quad f^{-1} \cdot g \in H}$
> -   $f \,_H \sim g \, \quad \iff \quad g \cdot f^{-1} \in H$

> [!lemma] Lemma 4.3.2: $\sim_H$ and $_H \sim$ are equivalence relations (p95)
> Let $(G, \cdot)$ be a group and $H \subseteq G$ a subgroup. Then the relations $\sim_H$ and $_H \sim$ are **equivalence relations** on $G$.

> [!lemma] Lemma 4.3.3 (p95)
> Let $(G, \cdot)$ be a group and $H \subseteq G$ a subgroup. For $f \in G$ we have
> $$\boxed{[f]_{\sim_H} = f \cdot H} \quad \text{ and } \quad [f]_{_H \sim} = H \cdot f$$

Now that we have identified left and right cosets **of** $H$ **in** $G$ as equivalence classes under $\sim_H$ and $_H \sim$, we can apply Theorem 1.3.3 (Properties of equivalence classes) to these equivalence relations:

> [!theorem] Theorem 4.3.4: Properties of cosets (p96)
> Let $(G, \cdot)$ be a group and $H \subseteq G$ a subgroup. Then the following holds:
>
> 1. $\forall f \in G$, $\boxed{f \in f \cdot H}$ and $f \in H \cdot f$ (reflexivity).
> 2. We have $G = \bigcup_{f \in G} (f \cdot H) = \bigcup_{f \in G} (H \cdot f)$ ($G$ is covered by all equivalence classes).
> 3. $\forall f,g \in G$,
>     - **either**
>         - $\boxed{f \cdot H = g \cdot H}$
>         - $\boxed{(f \cdot H) \cap (g \cdot H) = \emptyset}$
>     - Similarly, **either**
>         - $H \cdot f = H \cdot g$
>         - $(H \cdot f) \cap (H \cdot g) = \emptyset$.
> 4. $\forall f,g \in G :$
>     - $\boxed{f \cdot H = g \cdot H \iff f \sim_H g \,\iff f^{-1} \cdot g \in H}$
>     - $H \cdot f = H \cdot g \iff f \,_H \sim g \iff g \cdot f^{-1} \in H$.

Since $e \cdot H = \{e \cdot h \mid h \in H\} = H$, we see from part 4 of Theorem 4.3.4 that
$$H = f \cdot H \iff e \cdot H = f \cdot H \iff e \sim_H f \iff e^{-1} \cdot f \in H \iff f \in H$$
and similarly
$$H = H \cdot f \iff H \cdot e = H \cdot f \iff H \,_H \sim f \iff f \cdot e^{-1} \in H \iff f \in H$$

> [!deduction] Deduction: When is a coset equal to the subgroup? (p96)
> Let $(G, \cdot)$ be a group and $H \subseteq G$ a subgroup. Then for any $f \in G$, we have
> $$\boxed{f \cdot H = H \iff f \in H} \quad \text{ and } \quad H \cdot f = H \iff f \in H$$
> We call an element from a coset a **representative** of that coset.

Below, it is illustrated that **cosets $H \cdot f$ form a partition of the group $G$**:
![[cosets-partition.jpg]]

## 4.4 The order of a subgroup and of an element

> [!theorem] Theorem 4.4.1: Lagrange's Theorem (p98)
> Let $(G, \cdot)$ be a _finite_ group and $H \subseteq G$ a subgroup. Then
> $$\boxed{|H| \text{ divides } |G|}$$
> So **the order of a subgroup divides the order of the group**. More precisely,
> $$\boxed{|G| = [G:H] \cdot |H|}$$
> This theorem is called _Lagrange's Theorem_

> [!definition] Definition 4.4.2: index of a subgroup in a group (p98)
> Let $(G, \cdot)$ be a group and $H \subseteq G$ a subgroup. The number of left (or right) cosets of $H$ in $G$ is denoted by
> $$[G : H] = |G / H| \overset{\text{Thm. }4.4.1}{=} \frac{|G|}{|H|}$$
> and is called the **index of $H$ in $G$**

> [!proposition] Proposition 4.4.4: order of a group element (p98)
> Let $(G, \cdot)$ be a _finite_ group and let $g \in G$ be a group element. Then
>
> 1. $\boxed{\operatorname{ord}(g) \text{ divides } |G|}$
> 2. $\forall g \in G: \boxed{g^{|G|} = e}$

**Why**?

1.  This follows from Lemma 4.1.8, which says that $$\operatorname{ord}(g) = |\gen{g}|$$ and Theorem 4.4.1, which says that $$|\gen{g}| \text{ divides } |G| \qquad $$ since $\gen{g}$ is a (cyclic) subgroup of $G$.

2.  Because of part 1, we can write$$|G| = k \cdot \operatorname{ord}(g)$$for some integer $k$. This gives us$$g^{|G|} = g^{k \cdot \operatorname{ord}(g)} = (g^{\operatorname{ord}(g)})^k = e^k = e.$$

Proposition 4.4.4 has a number of interesting consequences for specific groups.

We start with **Euler's theorem**:

> [!corollary] Corollary 4.4.6: Euler's theorem (p99)
> Let $d,n \in \Z$ be two integers and assume that $\gcd(d,n) = 1$. Then
> $$d^{\phi(n)} \equiv 1 \pmod n$$
> where $\phi(n)$ is Euler's totient function defined by $\phi(n) = |(\Zn)^*|$.

In case $n$ is a prime number $p$, we have
$$\phi(p) = |\{i \in \{1, \ldots, p-1\} \mid \gcd(i,p) = 1\}| = p-1$$
This gives us the following special case of Euler's theorem, known as **Fermat's little theorem**:

> [!corollary] Corollary 4.4.7: Fermat's little theorem (p99)
> Let $p$ be a prime number and let $d \in \N$ such that $p \nmid d$. Then
> $$d^{p-1} \equiv 1 \pmod p$$
