## 6.1 Group homomorphisms

> [!definition] Definition 6.1.1: Group homomorphism and isomorphism
> Let $(G_1, \cdot_1)$ and $(G_2, \cdot_2)$ be groups. A function $\boxed{\psi: G_1 \to G_2}$ is a **group <u>homomorphism</u>** if it satisfies
>
> 1. $\boxed{\psi(e_1) = e_2}$
> 2. $\forall f,g \in G: \boxed{\psi(f \cdot_1 g) = \psi(f) \cdot_2 \psi(g)}$
>
> If $\psi : G_1 \to G_2$ is **bijective** as well, it is called a **group <u>isomorphism</u>**.

> [!definition] Isomorphic Groups
> Two groups $(G_1, \cdot_1)$ and $(G_2, \cdot_2)$ are called **isomorphic**
> if there exists a group isomorphism (bijective homomorphism) $\psi : G_1 \to G_2$:$$\boxed{(G_1, \cdot_1) \simeq (G_2, \cdot_2)}$$

> [!exercise] Exercise 6.18: Isomorphism as an equivalence relation
> Being isomorphic is an equivalence relation on the set of all groups.
>
> -   Reflexive:
>     -   _$\text{id}_G : G \to G$ is a group isomorphism (**automorphism**)._
> -   Symmetric
>     -   _If $\psi : G_1 \to G_2$ is a group isomorphism, then its inverse $\psi^{-1} : G_2 \to G_1$ is also a group isomorphism._
> -   Transitive:
>     -   _**The composition of two group homomorphisms is again a group homomorphism**._
>     -   $\psi_2 \circ \psi_1 : G_1 \to G_3$ is a group homomorphism if $\psi_1 : G_1 \to G_2$ and $\psi_2 : G_2 \to G_3$ are group homomorphisms.

![[images/6/multiplication-table.jpg]]
$$h = f \cdot_1 g \qquad \text{and} \qquad \psi(h) = \psi(f) \cdot_2 \psi(g)$$

Note how similar the definition of a group **homomorphism** is to the definition of a group **action** (Def. 5.1.1).

> [!example] Example 6.1.5: A group action is a group homomorphism
> Let $(G, \cdot)$ be a group with identity element $e_1$ that acts on the set $A$ via $\varphi : G \to S_A$.
>
> -   Since $\varphi_{e_1} = \text{id}_A$ and $\text{id}_A = e_2$ is the identity element of $S_A$, we have $\varphi(e_1) = e_2$.
> -   For any $f,g \in G$ we have $\varphi_{g \cdot f} = \varphi_g \circ \varphi_f$ by definition of a group action.
>     Since $\circ = \cdot_2$ is the group operation in $S_A$, we have $\varphi(g \cdot f) = \varphi(g) \cdot_2 \varphi(f)$.
>
> We conclude: **any group action $\varphi : G \to S_A$ is a group homomorphism on $S_A$**

Lemma 5.1.2 (group actions preserve inverses) can be generalized to any group **homomorphism**:

> [!lemma] Lemma 6.1.6: Group homomorphisms preserve inverses
> Let $\psi : G_1 \to G_2$ be a group homomorphism. Then for any $f \in G_1$ we have
> $$\boxed{\psi(f^{-1}) = (\psi(f))^{-1}}$$

> [!definition] Definition 6.1.7: Kernel of a group homomorphism
> Let $\psi : G_1 \to G_2$ be a group homomorphism and let $e_2$ be the identity element of $G_2$.
> Then we define the **kernel** of $\psi$ as
> $$\boxed{\ker(\psi) := \{ g \in G_1 \mid \psi(g) = e_2 \}}$$

> [!fact] Kernel of $\psi : G_1 \to G_2$ always contains the identity element of $G_1$
> Since $\psi$ is a group homomorphism, we have $\psi(e_1) = e_2$. Therefore $$e_1 \in \ker(\psi)$$

If the kernel only contains the identity element, the homomorphism $\psi$ is injective:

> [!lemma] Lemma 6.1.8: Injectivity and kernel
> Let $\psi : G_1 \to G_2$ be a group homomorphism. Then $$\boxed{\psi \text{ is injective} \iff \ker(\psi) = \{ e_1 \}}$$

We proved this in Exercise 6.14.

> [!fact] Group <u>iso</u>morphisms have trivial kernel
> If $\psi : G_1 \to G_2$ is a group **iso**morphism, then $\psi$ is bijective and therefore injective.
> By Lemma 6.1.8, we have $$\ker(\psi) = \{ e_1 \}$$

> [!theorem] Theorem 6.1.9: Kernel is a NORMAL subgroup
> Let $\psi : G_1 \to G_2$ be a group homomorphism. Then $$\ker(\psi) \subseteq G_1 \text{ is a subgroup of } G_1$$
> Moreover,
> $$\forall f \in G_1 : \qquad \boxed{f \cdot_1 \ker(\psi) = \ker(\psi) \cdot_1 f}$$
> In other words, the kernel is a **normal subgroup** of $G_1$ (Def. 6.1.10).

> [!definition] Definition 6.1.10: Normal subgroup
> A subgroup $H$ of a group $(G, \cdot)$ is called a **<u>normal</u> subgroup** if
> $$\forall f \in G : \qquad \boxed{f \cdot H = H \cdot f}$$
> In other words, all left cosets of $H$ are equal to the corresponding right cosets.

> [!deduction] The kernel is a normal subgroup
> It follows directly from Theorem 6.1.9 and Definition 6.1.10 that the **kernel** of any group homomorphism $\psi : G_1 \to G_2$ is a **normal** subgroup of $G_1$.

Because the **kernel is a normal subgroup**, we can prove that a subgroup $H$ of a group $G$ is normal by identifying it as the kernel of a suitable group homomorphism $\psi : G \to G_2$.

> [!definition] Definition: Image of a group homomorphism
> Let $\psi : G_1 \to G_2$ be a group homomorphism. Then we define the **image** of $\psi$ as
>
> $$
> \boxed{\text{im}(\psi) := \{ \psi(g) \mid g \in G_1 \} \subseteq G_2}
> $$

Note that the image is **never** **empty**, since $e_2$ is always in it:
$$e_1 \in G_1 \implies \psi(e_1) \eqDef \boxed{e_2 \in \text{im}(\psi)}.$$

> [!exercise] Exercise 6.15: The image is a subgroup of $G_2$
> Let $\psi : G_1 \to G_2$ be a group homomorphism. Then $$\text{im}(\psi) \subseteq G_2 \text{ is a subgroup of } G_2.$$

## 6.2 Quotient groups

We will show that a **normal** subgroup (with left cosets = right cosets) $H \subseteq G$ of a group $(G, \cdot)$ can be used to construct a new group, called the **quotient group** $G/H$.

> [!definition] Definition 6.2.1:
> Let $(G, \cdot)$ be a group and $H \subseteq G$ be a **normal** subgroup of $G$ we define
> $$\boxed{G/H := \{ f \cdot H \mid f \in G \}} = \{ H \cdot f \mid f \in G \}$$
> as the **set of all cosets** of $H$ in $G$.
> Its size $|G/H|$ is called the **index** of $H$ in $G$ and denoted by $[G : H]$.

Using multiplication of subsets (Def. 4.2.1), we can define a **group operation** $\cdot$ on $G/H$:$$(fH) \cdot (gH) := \{k \cdot \ell \mid k \in fH, \ell \in gH\}$$where $fH, gH \in G/H$.

> [!definition] Definition 6.2.2
> Let $(G, \cdot)$ be a group and $H \subseteq G$ be a <u>normal</u> subgroup of $(G, \cdot)$.
> Let $C,D \in G/H$ be two cosets of $H$ in $G$.
> Suppose that $f \in C$ and $g \in D$ are arbitrary representatives of $C$ and $D$, respectively.
>
> We define the **product** of the cosets $C$ and $D$ as
> $$C \cdot D := (f \cdot g)H$$
> Note that this coset is independent of the choice of representatives $f$ and $g$.

> [!notation] Notation: representatives of cosets
> If $C \in G/H$ is a coset of the normal subgroup $H$ in $G$, then any $f \in C$ is called a **representative** of the coset $C$.

> [!definition] Restated Definition 6.2.2
> If $f$ is a representative of a coset $C \in G/H$ and $g$ is a representative of a coset $D \in G/H$, then $C \cdot D$ is again a coset of $H$ in $G$ (and thus $C \cdot D \in G/H$) and $f \cdot g$ is a representative of $C \cdot D$.

> [!definition] Definition 6.2.3: Quotient group
> Let $(G, \cdot)$ be a group, $H \subseteq G$ a **normal** subgroup of $G$ and $G/H$ the set of all cosets of $H$ in $G$ (Def. 6.2.1). Then the multiplication of cosets$$\boxed{(fH) \cdot (gH) := (f \cdot g)H} \quad \textit{(Def. 6.2.2)}$$ gives rise to a **group structure** on $(G/H, \cdot)$.

We can explicitly write out the group operations to clarify how they work. Let $\cdot_G$ be the group operation in $(G, \cdot_G)$ (with **normal** subgroup $H$) and $\cdot_{G/H}$ be the group operation in the quotient group $(G/H, \cdot_{G/H})$. Then
$$(fH) \cdot_{G/H} (gH) = (f \cdot_G g)H.$$

We can see that

1. The composition of left (right) cosets is again a left (right) coset.
2. The representative of the composition is the composition of the representatives.

> [!exercise] Identity element of the quotient group
> Let $(G, \cdot)$ be a group, $H \subseteq G$ a **normal** subgroup of $G$ and $(G/H, \cdot)$ the quotient group.
>
> $$
> \boxed{e_{G/H} = H}
> $$

**Proof**

By definition of the identity element in a group, we have to show that
$$(fH) \cdot H = fH = H \cdot (fH)$$
Using the definition of the group operation in the quotient group, we have
$$(fH) \cdot H = (fH) \cdot (e_G H) \eqDef (f \cdot e_G)H = fH$$
and
$$H \cdot (fH) = (e_G H) \cdot (fH) \eqDef (e_G \cdot f)H = fH.$$

> [!exercise] Inverse of a left coset in the quotient group
> Let $(G, \cdot)$ be a group, $H \subseteq G$ a **normal** subgroup of $G$ and $(G/H, \cdot)$ the quotient group.
> $$ \forall f \in G : \qquad \boxed{(fH)^{-1} = (f^{-1})H} $$

**Proof**

By definition of the inverse element in a group, we have to show that
$$(fH) \cdot (f^{-1}H) = e_{G/H} = H = (H f^{-1}) \cdot (fH)$$
Using the definition of the group operation in the quotient group, we have
$$(fH) \cdot (f^{-1}H) = (f \cdot f^{-1})H = e_G H = H.$$
and the proof is completely analogous for the right side.

---

> [!exercise] Group Automorphisms
> A group isomorphism $\psi : G \to G$ from a group $(G, \cdot)$ to itself is called a **group automorphism**.
> The set of all group automorphisms of $(G, \cdot)$ is denoted by $\text{Aut}(G)$.
> $$(\text{Aut}(G), \circ) \text{ is a group}$$
> where $\circ$ is the composition of functions.

**Proof**

-   We already showed in Exercise 6.18 that the **composition of two group homomorphisms is again a group homomorphism.**
-   The identity function $\text{id}_G : G \to G$ is a group automorphism (Exercise 6.18).
-   The inverse of a group automorphism is again a group automorphism (Exercise 6.18).
-   Composition of functions is associative (function composition is associative by Lemma 2.1.2)
